isa/Halicore_Typecheck.thy
@@ -15,6 +15,8 @@ lemmas term_cont_rules =
   type_cont_rules
   cont_V_app cont_V_lam
   cont_T_app cont_T_abs
+  cont_cases cont_match cont_allmatch
+  cont_branch0 cont_branchV
 
 use "typecheck.ML"
 
